theories/Int63/vst/verif/vsu.v
@@ -1,0 +1,30 @@
+From VST Require Import floyd.proofauto.
+From VST Require Import floyd.VSU.
+
+From appliedfm Require Import Int63.vst.clightgen.int63.
+From appliedfm Require Import Int63.vst.spec.spec.
+From appliedfm Require Import Int63.vst.verif.verif.
+
+#[local] Existing Instance NullExtension.Espec.
+
+Lemma int63__vsu: VSU int63__specs.externs int63__specs.imports ltac:(QPprog prog) int63__specs.exports emp.
+Proof.
+  mkVSU prog int63__specs.exports.
+  - solve_SF_internal body_decode_int63.
+  - solve_SF_internal body_encode_int63.
+  - solve_SF_internal body_int63_zero.
+  - solve_SF_internal body_int63_one.
+  - solve_SF_internal body_int63_neg.
+  - solve_SF_internal body_int63_abs.
+  - solve_SF_internal body_int63_add.
+  - solve_SF_internal body_int63_sub.
+  - solve_SF_internal body_int63_mul.
+  - solve_SF_internal body_int63_div.
+  - solve_SF_internal body_int63_rem.
+  - solve_SF_internal body_int63_shiftl.
+  - solve_SF_internal body_int63_shiftr.
+  - solve_SF_internal body_int63_or.
+  - solve_SF_internal body_int63_and.
+  - solve_SF_internal body_int63_xor.
+  - solve_SF_internal body_int63_not.
+Qed.
